Trie: find

Bedrock/Platform/Facade/examples/Trie.v
@@ -25,6 +25,12 @@ Definition keepLen (ts : WSTuplSet) (key : W) (len : nat) : WSTuplSet :=
               /\ length bs = len.
 Definition empty (ts : WSTuplSet) := forall t, ~Ensembles.In _ ts t.
 
+Definition agreeUpto (key : nat) (ts : WSTuplSet) (posn : nat) (bs : list B) :=
+  forall i, (i < posn)%nat
+    -> forall t, ts t
+      -> exists cap bs', nth_error (indexedElement t) key = Some (WSBytes cap bs')
+                         /\ nth_error bs i = nth_error bs' i.
+
 
 Module Type ADT.
   Parameter trie : W -> W -> WSTuplSet -> W -> HProp.
@@ -69,16 +75,16 @@ Module Type ADT.
       -> tries len key sks ts posn p ===>
          Ex sk, Ex sks', Ex ch, Ex tp, Ex next,
            [| sks = sk :: sks' |]
-           * (p ==*> ch, tp, next)
-           * trie' len key sk (keepPosnEq ts key posn (WtoB ch)) (S posn) tp
-           * tries len key sks' (keepPosnNe ts key posn (WtoB ch)) posn next.
+           * (p ==*> BtoW ch, tp, next) * [| tp <> 0 |]
+           * trie' len key sk (keepPosnEq ts key posn ch) (S posn) tp
+           * tries len key sks' (keepPosnNe ts key posn ch) posn next.
   Axiom tries_cons_bwd : forall len key sks ts posn (p : W),
       p <> 0
       -> (Ex sk, Ex sks', Ex ch, Ex tp, Ex next,
            [| sks = sk :: sks' |]
-           * (p ==*> ch, tp, next)
-           * trie' len key sk (keepPosnEq ts key posn (WtoB ch)) (S posn) tp
-           * tries len key sks' (keepPosnNe ts key posn (WtoB ch)) posn next)
+           * (p ==*> BtoW ch, tp, next) * [| tp <> 0 |]
+           * trie' len key sk (keepPosnEq ts key posn ch) (S posn) tp
+           * tries len key sks' (keepPosnNe ts key posn ch) posn next)
          ===> tries len key sks ts posn p.
 End ADT.
 
@@ -95,9 +101,9 @@ Module Adt : ADT.
       | nil => [| p = 0 |] * [| empty ts |]
       | sk :: sks' => [| p <> 0 |]
                       * Ex ch, Ex tp, Ex next,
-                        (p ==*> ch, tp, next)
-                        * trie' sk (keepPosnEq ts key posn (WtoB ch)) tp
-                        * tries' sks' (keepPosnNe ts key posn (WtoB ch)) next
+                        (p ==*> BtoW ch, tp, next) * [| tp <> 0 |]
+                        * trie' sk (keepPosnEq ts key posn ch) tp
+                        * tries' sks' (keepPosnNe ts key posn ch) next
       end.
   End tries.
 
@@ -199,9 +205,9 @@ Module Adt : ADT.
       -> tries len key sks ts posn p ===>
          Ex sk, Ex sks', Ex ch, Ex tp, Ex next,
            [| sks = sk :: sks' |]
-           * (p ==*> ch, tp, next)
-           * trie' len key sk (keepPosnEq ts key posn (WtoB ch)) (S posn) tp
-           * tries len key sks' (keepPosnNe ts key posn (WtoB ch)) posn next.
+           * (p ==*> BtoW ch, tp, next) * [| tp <> 0 |]
+           * trie' len key sk (keepPosnEq ts key posn ch) (S posn) tp
+           * tries len key sks' (keepPosnNe ts key posn ch) posn next.
   Proof.
     destruct sks; sepLemma.
   Qed.
@@ -210,9 +216,9 @@ Module Adt : ADT.
       p <> 0
       -> (Ex sk, Ex sks', Ex ch, Ex tp, Ex next,
            [| sks = sk :: sks' |]
-           * (p ==*> ch, tp, next)
-           * trie' len key sk (keepPosnEq ts key posn (WtoB ch)) (S posn) tp
-           * tries len key sks' (keepPosnNe ts key posn (WtoB ch)) posn next)
+           * (p ==*> BtoW ch, tp, next) * [| tp <> 0 |]
+           * trie' len key sk (keepPosnEq ts key posn ch) (S posn) tp
+           * tries len key sks' (keepPosnNe ts key posn ch) posn next)
          ===> tries len key sks ts posn p.
   Proof.
     repeat sepLemma.
@@ -239,9 +245,10 @@ Definition insertS := SPEC("extra_stack", "self", "tup") reserving 21
     * [| insert ts t ts' |]
   POST[R] [| R = $0 |] * trie len key ts' (V "self") * mallocHeap 0.
 
-Definition findS := SPEC("extra_stack", "self", "k") reserving 34
+Definition findS := SPEC("extra_stack", "self", "k", "len") reserving 39
   Al len, Al key, Al ts, Al cap, Al bs,
   PRE[V] trie len key ts (V "self") * bytes cap bs (V "k") * mallocHeap 0
+         * [| wordToNat (V "len") = length bs |]
   POST[R] trie len key ts (V "self") * Ex ls, wlseq ls R
         * bytes cap bs (V "k") * mallocHeap 0
         * [| EnsembleIndexedListEquivalence (keepEq ts key bs) ls |].
@@ -252,15 +259,16 @@ Definition enumerateS := SPEC("extra_stack", "self") reserving 34
   POST[R] trie len key ts (V "self") * Ex ls, wlseq ls R * mallocHeap 0
           * [| EnsembleIndexedListEquivalence ts ls |].
 
-
 Definition m := bimport [[ "malloc"!"malloc" @ [mallocS], "malloc"!"free" @ [freeS],
-                           "WSTuple"!"get" @ [WSTuple.getS],
+                           "WSTuple"!"get" @ [WSTuple.getS], "ByteString"!"get" @ [ByteString.getS],
+                           "WsTupleList"!"new" @ [WsTupleList.newS],
                            "WsTuples0"!"new" @ [WsTuples0.newS], "WsTuples0"!"insert" @ [WsTuples0.insertS],
+                           "WsTuples0"!"enumerate" @ [WsTuples0.enumerateS],
                            "WsTuples0"!"enumerateInto" @ [WsTuples0.enumerateIntoS] ]]
   bmodule "Trie" {{
     bfunction "new"("extra_stack", "len", "key") [newS]
-      "extra_stack" <-- Call "malloc"!"malloc"(0, 2)
-      [PRE[V, R] R =?> 2 * [| R <> 0 |] * [| freeable R 2 |]
+      "extra_stack" <-- Call "malloc"!"malloc"(0, 3)
+      [PRE[V, R] R =?> 3 * [| R <> 0 |] * [| freeable R 3 |]
               * [| (V "len" >= $2)%word |] * [| (V "key" < V "len")%word |]
        POST[R'] trie (V "len") (V "key") Empty R'];;
 
@@ -268,6 +276,93 @@ Definition m := bimport [[ "malloc"!"malloc" @ [mallocS], "malloc"!"free" @ [fre
       "extra_stack" + 4 *<- "key";;
       "extra_stack" + 8 *<- 0;;
       Return "extra_stack"
+    end
+
+    with bfunction "find"("extra_stack", "self", "k", "len", "key", "posn", "ch", "ch2", "stop") [findS]
+      "key" <-* "self" + 4;;
+      "self" <-* "self" + 8;;
+      "posn" <- 0;;
+
+      [Al len, Al key, Al ts, Al cap, Al bs, Al sk,
+       PRE[V] trie' len key sk ts (wordToNat (V "posn")) (V "self") * bytes cap bs (V "k") * mallocHeap 0
+         * [| wordToNat (V "len") = length bs |] * [| V "posn" <= V "len" |]%word
+         * [| agreeUpto (wordToNat key) ts (wordToNat (V "posn")) bs |]
+       POST[R] trie' len key sk ts (wordToNat (V "posn")) (V "self") * Ex ls, wlseq ls R
+         * bytes cap bs (V "k") * mallocHeap 0
+         * [| EnsembleIndexedListEquivalence (keepEq ts key bs) ls |]]
+      While ("self" <> 0) {
+        If ("posn" = "len") {
+          (* We've consumed all characters in the key, so it's now or never.
+           * We need to return whatever is associated with this node. *)
+          "self" <-* "self";;
+          "self" <-- Call "WsTuples0"!"enumerate"("extra_stack", "self")
+          [PRE[_, R] Emp
+           POST[R'] [| R' = R |] ];;
+          Return "self"
+        } else {
+          (* In the list of possible next characters, find the one that matches
+           * this position in the key. *)
+          "ch" <-- Call "ByteString"!"get"("extra_stack", "k", "posn")
+          [Al len, Al key, Al ts, Al cap, Al bs, Al sk,
+           PRE[V, R] trie' len key sk ts (wordToNat (V "posn")) (V "self") * bytes cap bs (V "k") * mallocHeap 0
+             * [| wordToNat (V "len") = length bs |] * [| V "posn" < V "len" |]%word
+             * [| V "self" <> 0 |] * [| R = BtoW (nth (wordToNat (V "posn")) bs (wzero _)) |]
+             * [| agreeUpto (wordToNat key) ts (wordToNat (V "posn")) bs |]
+
+           POST[R'] trie' len key sk ts (wordToNat (V "posn")) (V "self") * Ex ls, wlseq ls R'
+             * bytes cap bs (V "k") * mallocHeap 0
+             * [| EnsembleIndexedListEquivalence (keepEq ts key bs) ls |]];;
+
+          "self" <-* "self" + 4;;
+          "stop" <- 0;;
+          [Al len, Al key, Al ts, Al cap, Al bs, Al sks,
+           PRE[V] bytes cap bs (V "k") * mallocHeap 0
+             * tries len key sks ts (wordToNat (V "posn")) (V "self")
+             * [| wordToNat (V "len") = length bs |] * [| V "posn" < V "len" |]%word
+             * [| V "ch" = BtoW (nth (wordToNat (V "posn")) bs (wzero _)) |]
+             * [| agreeUpto (wordToNat key) ts (wordToNat (V "posn")) bs |]
+           POST[R] Ex ls, wlseq ls R
+             * bytes cap bs (V "k") * mallocHeap 0
+             * tries len key sks ts (wordToNat (V "posn")) (V "self")
+             * [| EnsembleIndexedListEquivalence (keepEq ts key bs) ls |]]
+          While ("stop" = 0) {
+            If ("self" = 0) {
+              "stop" <- 1
+            } else {
+              "ch2" <-* "self";;
+              If ("ch" = "ch2") {
+                (* Found a match! *)
+                "stop" <- 1
+              } else {
+                "self" <-* "self" + 8
+              }
+            }
+          };;
+
+          If ("self" = 0) {
+            (* No match for the next character, so we give up. *)
+            "self" <-- Call "WsTupleList"!"new"("extra_stack")
+            [PRE[_, R] Emp
+             POST[R'] [| R' = R |] ];;
+            Return "self"
+          } else {
+            "ch2" <-* "self";;
+            If ("ch" = "ch2") {
+              (* Reconfirmed the match.
+               * (The code is structured this way to make the proof easier.) *)
+              "self" <-* "self" + 4;;
+              "posn" <- 1 + "posn"
+            } else {
+              Diverge (* Should be impossible, but we aren't proving it now. *)
+            }
+          }
+        }
+      };;
+
+      "self" <-- Call "WsTupleList"!"new"("extra_stack")
+      [PRE[_, R] Emp
+      POST[R'] [| R' = R |] ];;
+      Return "self"
     end
   }}.
 
@@ -280,7 +375,276 @@ Qed.
 
 Hint Resolve empty_Empty.
 
-Ltac t := sep_auto; eauto.
+Lemma agreeUpto_zero : forall key ts bs,
+    agreeUpto key ts 0 bs.
+Proof.
+  unfold agreeUpto; intuition.
+Qed.
+
+Local Hint Immediate agreeUpto_zero.
+
+Lemma increment : forall posn : W,
+    (exists len, posn < len)
+    -> wordToNat (natToW 1 ^+ posn) = S (wordToNat posn).
+Proof.
+  firstorder.
+  rewrite wplus_comm.
+  erewrite <- next.
+  omega.
+  eassumption.
+Qed.
+
+Hint Rewrite increment using (eexists; eassumption) : sepFormula.
+
+Lemma oneplus_bound : forall posn len,
+    posn < len
+    -> natToW 1 ^+ posn <= len.
+Proof.
+  intros.
+  pre_nomega.
+  rewrite wplus_comm.
+  erewrite <- next.
+  omega.
+  pre_nomega.
+  eassumption.
+Qed.
+
+Local Hint Immediate oneplus_bound.
+
+Lemma nth_error_nth : forall A (d : A) n ls,
+    (n < length ls)%nat
+    -> nth_error ls n = Some (nth n ls d).
+Proof.
+  induction n; destruct ls; simpl; intuition.
+Qed.
+
+Lemma agreeUpto_keepPosnEq : forall key ts (posn : W) ch ch' bs len,
+    agreeUpto (wordToNat key) ts (wordToNat posn) bs
+    -> ch' = BtoW ch
+    -> ch' = BtoW (nth (wordToNat posn) bs (wzero 8))
+    -> posn < len
+    -> wordToNat len = length bs
+    -> agreeUpto (wordToNat key) (keepPosnEq ts key (wordToNat posn) ch) (S (wordToNat posn)) bs.
+Proof.
+  unfold agreeUpto, keepPosnEq; intuition.
+  destruct H7 as [ ? [ ] ]; intuition.
+  do 2 eexists; split; eauto.
+  Require Import Arith.
+  destruct (eq_nat_dec i (wordToNat posn)); subst.
+
+  apply (f_equal WtoB) in H1.
+  repeat erewrite BtoW_WtoB in H1 by reflexivity.
+  subst.
+  erewrite nth_error_nth.
+  eauto.
+  nomega.
+
+  eapply H in H6.
+  destruct H6 as [ ? [ ? [ ] ] ].
+  rewrite H7 in H0.
+  inversion_clear H0.
+  eassumption.
+  omega.
+Qed.
+
+Local Hint Immediate agreeUpto_keepPosnEq.
+
+Lemma EnsembleIndexedListEquivalence_cong : forall A (ts ts' : @IndexedEnsemble A) ls,
+    EnsembleIndexedListEquivalence ts ls
+    -> (forall x, ts x <-> ts' x)
+    -> EnsembleIndexedListEquivalence ts' ls.
+Proof.
+  unfold EnsembleIndexedListEquivalence.
+  firstorder.
+Qed.
+
+Lemma keepEq_keepPosnEq : forall ts ch ch' (posn len : W) ls key bs,
+    EnsembleIndexedListEquivalence
+      (keepEq (keepPosnEq ts key (wordToNat posn) ch') key bs) ls
+    -> ch = BtoW ch'
+    -> ch = BtoW (nth (wordToNat posn) bs (wzero 8))
+    -> wordToNat len = length bs
+    -> posn < len
+    -> EnsembleIndexedListEquivalence (keepEq ts key bs) ls.
+Proof.
+  intros.
+  eapply EnsembleIndexedListEquivalence_cong.
+  eassumption.
+  unfold keepEq, keepPosnEq, Ensembles.In; subst; intuition.
+  destruct H5.
+  do 2 eexists; split; eauto.
+  apply (f_equal WtoB) in H1.
+  erewrite BtoW_WtoB in H1 by reflexivity.
+  subst.
+  erewrite nth_error_nth.
+  f_equal.
+  erewrite BtoW_WtoB by reflexivity.
+  eauto.
+  pre_nomega.
+  rewrite H2 in H3.
+  assumption.
+Qed.
+
+Local Hint Immediate keepEq_keepPosnEq.
+
+Lemma agreeUpto_equal' : forall (bs1 bs2 : list B),
+    (forall i, (i < length bs1)%nat
+               -> nth_error bs1 i = nth_error bs2 i)
+    -> length bs1 = length bs2
+    -> bs1 = bs2.
+Proof.
+  induction bs1; destruct bs2; simpl; intuition.
+  assert (0 < S (length bs1))%nat by omega.
+  generalize (H 0); simpl; intuition.
+  inversion_clear H3.
+  f_equal.
+  apply IHbs1; intuition.
+  apply (H (S i)); auto.
+Qed.
+
+Lemma agreeUpto_equal : forall key ts t bs1 bs2 cap,
+    agreeUpto key ts (length bs1) bs1
+    -> length bs1 = length bs2
+    -> ts t
+    -> nth_error (indexedElement t) key = Some (WSBytes cap bs2)
+    -> bs1 = bs2.
+Proof.
+  unfold agreeUpto; intros.
+  eapply agreeUpto_equal'.
+  intros.
+  eapply H in H3; try eassumption.
+  destruct H3 as [ ? [ ] ]; intuition.
+  rewrite H2 in H4; inversion_clear H4.
+  assumption.
+  assumption.
+Qed.
+
+Lemma keepLen_keepEq : forall ts (posn len : W) ls key bs,
+    EnsembleIndexedListEquivalence (keepLen ts key (wordToNat posn)) ls
+    -> posn = len
+    -> wordToNat len = length bs
+    -> agreeUpto (wordToNat key) ts (wordToNat posn) bs
+    -> EnsembleIndexedListEquivalence (keepEq ts key bs) ls.
+Proof.
+  intros.
+  eapply EnsembleIndexedListEquivalence_cong.
+  eassumption.
+  unfold keepEq, keepLen, Ensembles.In; subst; intuition.
+
+  destruct H4 as [ ? [ ] ]; intuition.
+  replace x1 with bs in H4.
+  eauto.
+  eapply agreeUpto_equal; eauto.
+  rewrite <- H1.
+  assumption.
+
+  firstorder.
+Qed.
+
+Local Hint Immediate keepLen_keepEq.
+
+Lemma length_bound : forall (posn : W) len len',
+    posn <> len'
+    -> posn <= len'
+    -> wordToNat len' = len
+    -> (wordToNat posn < len)%nat.
+Proof.
+  intros; subst.
+  pre_nomega.
+  apply Bootstrap.wordToNat_ninj in H.
+  omega.
+Qed.
+
+Local Hint Immediate length_bound.
+
+Lemma length_bound' : forall (posn : W) len,
+    posn <> len
+    -> posn <= len
+    -> posn < len.
+Proof.
+  intros; subst.
+  pre_nomega.
+  apply Bootstrap.wordToNat_ninj in H.
+  omega.
+Qed.
+
+Local Hint Immediate length_bound'.
+
+Lemma agreeUpto_keepPosnNe : forall key ts (posn : W) ch ch' bs len,
+    agreeUpto (wordToNat key) ts (wordToNat posn) bs
+    -> ch = BtoW (nth (wordToNat posn) bs (wzero _))
+    -> ch <> BtoW ch'
+    -> posn < len
+    -> wordToNat len = length bs
+    -> agreeUpto (wordToNat key) (keepPosnNe ts key (wordToNat posn) ch') (wordToNat posn) bs.
+Proof.
+  unfold agreeUpto, keepPosnNe; intuition.
+Qed.
+
+Local Hint Immediate agreeUpto_keepPosnNe.
+
+Lemma keepEq_keepPosnNe : forall ts ch ch' (posn len : W) ls key bs,
+    EnsembleIndexedListEquivalence
+      (keepEq (keepPosnNe ts key (wordToNat posn) ch') key bs) ls
+    -> ch = BtoW (nth (wordToNat posn) bs (wzero 8))
+    -> ch <> BtoW ch'
+    -> wordToNat len = length bs
+    -> posn < len
+    -> EnsembleIndexedListEquivalence (keepEq ts key bs) ls.
+Proof.
+  intros.
+  eapply EnsembleIndexedListEquivalence_cong.
+  eassumption.
+  unfold keepEq, keepPosnNe, Ensembles.In; subst; intuition.
+  destruct H5.
+  do 2 eexists; split; eauto.
+  intro.
+  erewrite nth_error_nth in H5.
+  inversion H5; clear H5.
+  apply H1.
+  apply (f_equal BtoW) in H7.
+  eauto.
+  pre_nomega.
+  rewrite H2 in H3.
+  assumption.
+Qed.
+
+Local Hint Immediate keepEq_keepPosnNe.
+
+Lemma keepEq_empty : forall ts key bs,
+    empty ts
+    -> EnsembleIndexedListEquivalence (keepEq ts key bs) nil.
+Proof.
+  unfold EnsembleIndexedListEquivalence, UnConstrFreshIdx, UnIndexedEnsembleListEquivalence, keepEq, Ensembles.In.
+  firstorder.
+  exact 0.
+  exists nil; simpl; firstorder.
+  constructor.
+Qed.
+
+Local Hint Immediate keepEq_empty.
+
+Ltac unifyLocals :=
+  match goal with
+  | [ _ : interp _ (![?P1] ?x) |- interp _ (![?P2] ?x) ] =>
+    match P1 with
+    | context[locals _ ?vs1 ?y _] =>
+      match P2 with
+      | context[locals _ ?vs2 y _] => unify vs1 vs2; descend
+      end
+    end
+  | [ |- interp _ (![?P1] ?x ---> ![?P2] ?x)%PropX ] =>
+    match P1 with
+    | context[locals ?y ?vs1 _ _] =>
+      match P2 with
+      | context[locals y ?vs2 _ _] => unify vs1 vs2; descend
+      end
+    end
+  end.
+
+Ltac t := solve [ enterFunction
+                  || (post; evaluate hints; try evaluate hints; descend; try unifyLocals;
+                      repeat (step hints; descend); eauto; cbv beta; congruence) ].
 
 Theorem ok : moduleOk m.
 Proof.
@@ -291,8 +655,50 @@ Proof.
   t.
   t.
   t.
+  t.
+  t.
+  t.
 
-  vcgen; try abstract t; t.
+  t.
+  t.
+  t.
+  t.
+  t.
+  t.
+  t.
+  t.
+  t.
+  t.
+  t.
+  t.
+  t.
+  t.
+  t.
+  t.
+  t.
+  t.
+  t.
+  t.
+  t.
+  t.
+  t.
+  t.
+  t.
+  t.
+  t.
+  t.
+  t.
+  t.
+  t.
+  t.
+  t.
+  t.
+  t.
+  t.
+  t.
+  t.
+  t.
+  t.
 
   Grab Existential Variables.
   exact 0.
